work related to global var and external fun

compiler_test/beepl_test/tcp1.ml
@@ -91,18 +91,21 @@ module Coq_Pos =
 
   let rec add x0 y0 =
     match x0 with
-    | XI p -> (match y0 with
-               | XI q -> XO (add_carry p q)
-               | XO q -> XI (add p q)
-               | XH -> XO (succ p))
-    | XO p -> (match y0 with
-               | XI q -> XI (add p q)
-               | XO q -> XO (add p q)
-               | XH -> XI p)
-    | XH -> (match y0 with
-             | XI q -> XO (succ q)
-             | XO q -> XI q
-             | XH -> XO XH)
+    | XI p ->
+      (match y0 with
+       | XI q -> XO (add_carry p q)
+       | XO q -> XI (add p q)
+       | XH -> XO (succ p))
+    | XO p ->
+      (match y0 with
+       | XI q -> XI (add p q)
+       | XO q -> XO (add p q)
+       | XH -> XI p)
+    | XH ->
+      (match y0 with
+       | XI q -> XO (succ q)
+       | XO q -> XI q
+       | XH -> XO XH)
 
   (** val add_carry : positive -> positive -> positive **)
 
@@ -113,14 +116,16 @@ module Coq_Pos =
        | XI q -> XI (add_carry p q)
        | XO q -> XO (add_carry p q)
        | XH -> XI (succ p))
-    | XO p -> (match y0 with
-               | XI q -> XO (add_carry p q)
-               | XO q -> XI (add p q)
-               | XH -> XO (succ p))
-    | XH -> (match y0 with
-             | XI q -> XI (succ q)
-             | XO q -> XO (succ q)
-             | XH -> XI XH)
+    | XO p ->
+      (match y0 with
+       | XI q -> XO (add_carry p q)
+       | XO q -> XI (add p q)
+       | XH -> XO (succ p))
+    | XH ->
+      (match y0 with
+       | XI q -> XI (succ q)
+       | XO q -> XO (succ q)
+       | XH -> XI XH)
 
   (** val pred_double : positive -> positive **)
 
@@ -231,18 +236,21 @@ module Coq_Pos =
   | XO p0 -> succ (size p0)
   | XH -> XH
 
-  (** val compare_cont : comparison -> positive -> positive -> comparison **)
+  (** val compare_cont :
+      comparison -> positive -> positive -> comparison **)
 
   let rec compare_cont r0 x0 y0 =
     match x0 with
-    | XI p -> (match y0 with
-               | XI q -> compare_cont r0 p q
-               | XO q -> compare_cont Gt p q
-               | XH -> Gt)
-    | XO p -> (match y0 with
-               | XI q -> compare_cont Lt p q
-               | XO q -> compare_cont r0 p q
-               | XH -> Gt)
+    | XI p ->
+      (match y0 with
+       | XI q -> compare_cont r0 p q
+       | XO q -> compare_cont Gt p q
+       | XH -> Gt)
+    | XO p ->
+      (match y0 with
+       | XI q -> compare_cont Lt p q
+       | XO q -> compare_cont r0 p q
+       | XH -> Gt)
     | XH -> (match y0 with
              | XH -> r0
              | _ -> Lt)
@@ -268,14 +276,16 @@ module Coq_Pos =
 
   let rec coq_lor p q =
     match p with
-    | XI p0 -> (match q with
-                | XI q0 -> XI (coq_lor p0 q0)
-                | XO q0 -> XI (coq_lor p0 q0)
-                | XH -> p)
-    | XO p0 -> (match q with
-                | XI q0 -> XI (coq_lor p0 q0)
-                | XO q0 -> XO (coq_lor p0 q0)
-                | XH -> XI p0)
+    | XI p0 ->
+      (match q with
+       | XI q0 -> XI (coq_lor p0 q0)
+       | XO q0 -> XI (coq_lor p0 q0)
+       | XH -> p)
+    | XO p0 ->
+      (match q with
+       | XI q0 -> XI (coq_lor p0 q0)
+       | XO q0 -> XO (coq_lor p0 q0)
+       | XH -> XI p0)
     | XH -> (match q with
              | XO q0 -> XI q0
              | _ -> q)
@@ -330,21 +340,24 @@ module Coq_Pos =
        | XI q0 -> coq_Nsucc_double (coq_lxor p0 q0)
        | XO q0 -> coq_Ndouble (coq_lxor p0 q0)
        | XH -> Npos (XI p0))
-    | XH -> (match q with
-             | XI q0 -> Npos (XO q0)
-             | XO q0 -> Npos (XI q0)
-             | XH -> N0)
+    | XH ->
+      (match q with
+       | XI q0 -> Npos (XO q0)
+       | XO q0 -> Npos (XI q0)
+       | XH -> N0)
 
   (** val testbit : positive -> n -> bool **)
 
   let rec testbit p n0 =
     match p with
-    | XI p0 -> (match n0 with
-                | N0 -> True
-                | Npos n1 -> testbit p0 (pred_N n1))
-    | XO p0 -> (match n0 with
-                | N0 -> False
-                | Npos n1 -> testbit p0 (pred_N n1))
+    | XI p0 ->
+      (match n0 with
+       | N0 -> True
+       | Npos n1 -> testbit p0 (pred_N n1))
+    | XO p0 ->
+      (match n0 with
+       | N0 -> False
+       | Npos n1 -> testbit p0 (pred_N n1))
     | XH -> (match n0 with
              | N0 -> True
              | Npos _ -> False)
@@ -398,9 +411,10 @@ module N =
     | Npos n' ->
       (match m with
        | N0 -> n0
-       | Npos m' -> (match Coq_Pos.sub_mask n' m' with
-                     | Coq_Pos.IsPos p -> Npos p
-                     | _ -> N0))
+       | Npos m' ->
+         (match Coq_Pos.sub_mask n' m' with
+          | Coq_Pos.IsPos p -> Npos p
+          | _ -> N0))
 
   (** val compare : n -> n -> comparison **)
 
@@ -409,9 +423,10 @@ module N =
     | N0 -> (match m with
              | N0 -> Eq
              | Npos _ -> Lt)
-    | Npos n' -> (match m with
-                  | N0 -> Gt
-                  | Npos m' -> Coq_Pos.compare n' m')
+    | Npos n' ->
+      (match m with
+       | N0 -> Gt
+       | Npos m' -> Coq_Pos.compare n' m')
 
   (** val leb : n -> n -> bool **)
 
@@ -439,27 +454,30 @@ module N =
     | XH ->
       (match b with
        | N0 -> Pair (N0, (Npos XH))
-       | Npos p -> (match p with
-                    | XH -> Pair ((Npos XH), N0)
-                    | _ -> Pair (N0, (Npos XH))))
+       | Npos p ->
+         (match p with
+          | XH -> Pair ((Npos XH), N0)
+          | _ -> Pair (N0, (Npos XH))))
 
   (** val coq_lor : n -> n -> n **)
 
   let coq_lor n0 m =
     match n0 with
     | N0 -> m
-    | Npos p -> (match m with
-                 | N0 -> n0
-                 | Npos q -> Npos (Coq_Pos.coq_lor p q))
+    | Npos p ->
+      (match m with
+       | N0 -> n0
+       | Npos q -> Npos (Coq_Pos.coq_lor p q))
 
   (** val coq_land : n -> n -> n **)
 
   let coq_land n0 m =
     match n0 with
     | N0 -> N0
-    | Npos p -> (match m with
-                 | N0 -> N0
-                 | Npos q -> Coq_Pos.coq_land p q)
+    | Npos p ->
+      (match m with
+       | N0 -> N0
+       | Npos q -> Coq_Pos.coq_land p q)
 
   (** val ldiff : n -> n -> n **)
 
@@ -475,9 +493,10 @@ module N =
   let coq_lxor n0 m =
     match n0 with
     | N0 -> m
-    | Npos p -> (match m with
-                 | N0 -> n0
-                 | Npos q -> Coq_Pos.coq_lxor p q)
+    | Npos p ->
+      (match m with
+       | N0 -> n0
+       | Npos q -> Coq_Pos.coq_lxor p q)
 
   (** val testbit : n -> n -> bool **)
 
@@ -542,10 +561,11 @@ module Z =
        | XI q -> pred_double (pos_sub p q)
        | XO q -> double (pos_sub p q)
        | XH -> Zpos (Coq_Pos.pred_double p))
-    | XH -> (match y0 with
-             | XI q -> Zneg (XO q)
-             | XO q -> Zneg (Coq_Pos.pred_double q)
-             | XH -> Z0)
+    | XH ->
+      (match y0 with
+       | XI q -> Zneg (XO q)
+       | XO q -> Zneg (Coq_Pos.pred_double q)
+       | XH -> Z0)
 
   (** val add : z -> z -> z **)
 
@@ -604,12 +624,14 @@ module Z =
              | Z0 -> Eq
              | Zpos _ -> Lt
              | Zneg _ -> Gt)
-    | Zpos x' -> (match y0 with
-                  | Zpos y' -> Coq_Pos.compare x' y'
-                  | _ -> Gt)
-    | Zneg x' -> (match y0 with
-                  | Zneg y' -> compOpp (Coq_Pos.compare x' y')
-                  | _ -> Lt)
+    | Zpos x' ->
+      (match y0 with
+       | Zpos y' -> Coq_Pos.compare x' y'
+       | _ -> Gt)
+    | Zneg x' ->
+      (match y0 with
+       | Zneg y' -> compOpp (Coq_Pos.compare x' y')
+       | _ -> Lt)
 
   (** val leb : z -> z -> bool **)
 
@@ -653,13 +675,15 @@ module Z =
       let r' = add (mul (Zpos (XO XH)) r0) (Zpos XH) in
       (match ltb r' b with
        | True -> Pair ((mul (Zpos (XO XH)) q), r')
-       | False -> Pair ((add (mul (Zpos (XO XH)) q) (Zpos XH)), (sub r' b)))
+       | False ->
+         Pair ((add (mul (Zpos (XO XH)) q) (Zpos XH)), (sub r' b)))
     | XO a' ->
       let Pair (q, r0) = pos_div_eucl a' b in
       let r' = mul (Zpos (XO XH)) r0 in
       (match ltb r' b with
        | True -> Pair ((mul (Zpos (XO XH)) q), r')
-       | False -> Pair ((add (mul (Zpos (XO XH)) q) (Zpos XH)), (sub r' b)))
+       | False ->
+         Pair ((add (mul (Zpos (XO XH)) q) (Zpos XH)), (sub r' b)))
     | XH ->
       (match leb (Zpos (XO XH)) b with
        | True -> Pair (Z0, (Zpos XH))
@@ -687,7 +711,9 @@ module Z =
          (match r0 with
           | Z0 -> Pair ((opp q), Z0)
           | _ -> Pair ((opp (add q (Zpos XH))), (sub b r0)))
-       | Zneg b' -> let Pair (q, r0) = pos_div_eucl a' (Zpos b') in Pair (q, (opp r0)))
+       | Zneg b' ->
+         let Pair (q, r0) = pos_div_eucl a' (Zpos b') in
+         Pair (q, (opp r0)))
 
   (** val div : z -> z -> z **)
 
@@ -707,14 +733,21 @@ module Z =
     | Zpos a0 ->
       (match b with
        | Z0 -> Pair (Z0, a)
-       | Zpos b0 -> let Pair (q, r0) = N.pos_div_eucl a0 (Npos b0) in Pair ((of_N q), (of_N r0))
-       | Zneg b0 -> let Pair (q, r0) = N.pos_div_eucl a0 (Npos b0) in Pair ((opp (of_N q)), (of_N r0)))
+       | Zpos b0 ->
+         let Pair (q, r0) = N.pos_div_eucl a0 (Npos b0) in
+         Pair ((of_N q), (of_N r0))
+       | Zneg b0 ->
+         let Pair (q, r0) = N.pos_div_eucl a0 (Npos b0) in
+         Pair ((opp (of_N q)), (of_N r0)))
     | Zneg a0 ->
       (match b with
        | Z0 -> Pair (Z0, a)
        | Zpos b0 ->
-         let Pair (q, r0) = N.pos_div_eucl a0 (Npos b0) in Pair ((opp (of_N q)), (opp (of_N r0)))
-       | Zneg b0 -> let Pair (q, r0) = N.pos_div_eucl a0 (Npos b0) in Pair ((of_N q), (opp (of_N r0))))
+         let Pair (q, r0) = N.pos_div_eucl a0 (Npos b0) in
+         Pair ((opp (of_N q)), (opp (of_N r0)))
+       | Zneg b0 ->
+         let Pair (q, r0) = N.pos_div_eucl a0 (Npos b0) in
+         Pair ((of_N q), (opp (of_N r0))))
 
   (** val quot : z -> z -> z **)
 
@@ -749,10 +782,11 @@ module Z =
   (** val log2 : z -> z **)
 
   let log2 = function
-  | Zpos p0 -> (match p0 with
-                | XI p -> Zpos (Coq_Pos.size p)
-                | XO p -> Zpos (Coq_Pos.size p)
-                | XH -> Z0)
+  | Zpos p0 ->
+    (match p0 with
+     | XI p -> Zpos (Coq_Pos.size p)
+     | XO p -> Zpos (Coq_Pos.size p)
+     | XH -> Z0)
   | _ -> Z0
 
   (** val testbit : z -> z -> bool **)
@@ -787,12 +821,17 @@ module Z =
       (match b with
        | Z0 -> a
        | Zpos b0 -> Zpos (Coq_Pos.coq_lor a0 b0)
-       | Zneg b0 -> Zneg (N.succ_pos (N.ldiff (Coq_Pos.pred_N b0) (Npos a0))))
+       | Zneg b0 ->
+         Zneg (N.succ_pos (N.ldiff (Coq_Pos.pred_N b0) (Npos a0))))
     | Zneg a0 ->
       (match b with
        | Z0 -> a
-       | Zpos b0 -> Zneg (N.succ_pos (N.ldiff (Coq_Pos.pred_N a0) (Npos b0)))
-       | Zneg b0 -> Zneg (N.succ_pos (N.coq_land (Coq_Pos.pred_N a0) (Coq_Pos.pred_N b0))))
+       | Zpos b0 ->
+         Zneg (N.succ_pos (N.ldiff (Coq_Pos.pred_N a0) (Npos b0)))
+       | Zneg b0 ->
+         Zneg
+           (N.succ_pos
+             (N.coq_land (Coq_Pos.pred_N a0) (Coq_Pos.pred_N b0))))
 
   (** val coq_land : z -> z -> z **)
 
@@ -808,7 +847,10 @@ module Z =
       (match b with
        | Z0 -> Z0
        | Zpos b0 -> of_N (N.ldiff (Npos b0) (Coq_Pos.pred_N a0))
-       | Zneg b0 -> Zneg (N.succ_pos (N.coq_lor (Coq_Pos.pred_N a0) (Coq_Pos.pred_N b0))))
+       | Zneg b0 ->
+         Zneg
+           (N.succ_pos
+             (N.coq_lor (Coq_Pos.pred_N a0) (Coq_Pos.pred_N b0))))
 
   (** val coq_lxor : z -> z -> z **)
 
@@ -819,12 +861,15 @@ module Z =
       (match b with
        | Z0 -> a
        | Zpos b0 -> of_N (Coq_Pos.coq_lxor a0 b0)
-       | Zneg b0 -> Zneg (N.succ_pos (N.coq_lxor (Npos a0) (Coq_Pos.pred_N b0))))
+       | Zneg b0 ->
+         Zneg (N.succ_pos (N.coq_lxor (Npos a0) (Coq_Pos.pred_N b0))))
     | Zneg a0 ->
       (match b with
        | Z0 -> a
-       | Zpos b0 -> Zneg (N.succ_pos (N.coq_lxor (Coq_Pos.pred_N a0) (Npos b0)))
-       | Zneg b0 -> of_N (N.coq_lxor (Coq_Pos.pred_N a0) (Coq_Pos.pred_N b0)))
+       | Zpos b0 ->
+         Zneg (N.succ_pos (N.coq_lxor (Coq_Pos.pred_N a0) (Npos b0)))
+       | Zneg b0 ->
+         of_N (N.coq_lxor (Coq_Pos.pred_N a0) (Coq_Pos.pred_N b0)))
 
   (** val eq_dec : z -> z -> sumbool **)
 
@@ -833,12 +878,14 @@ module Z =
     | Z0 -> (match y0 with
              | Z0 -> Left
              | _ -> Right)
-    | Zpos x1 -> (match y0 with
-                  | Zpos p0 -> Coq_Pos.eq_dec x1 p0
-                  | _ -> Right)
-    | Zneg x1 -> (match y0 with
-                  | Zneg p0 -> Coq_Pos.eq_dec x1 p0
-                  | _ -> Right)
+    | Zpos x1 ->
+      (match y0 with
+       | Zpos p0 -> Coq_Pos.eq_dec x1 p0
+       | _ -> Right)
+    | Zneg x1 ->
+      (match y0 with
+       | Zneg p0 -> Coq_Pos.eq_dec x1 p0
+       | _ -> Right)
  end
 
 (** val z_lt_dec : z -> z -> sumbool **)
@@ -937,12 +984,14 @@ let zshiftin b x0 =
 (** val zzero_ext : z -> z -> z **)
 
 let zzero_ext n0 x0 =
-  Z.iter n0 (fun rec0 x1 -> zshiftin (Z.odd x1) (rec0 (Z.div2 x1))) (fun _ -> Z0) x0
+  Z.iter n0 (fun rec0 x1 -> zshiftin (Z.odd x1) (rec0 (Z.div2 x1)))
+    (fun _ -> Z0) x0
 
 (** val zsign_ext : z -> z -> z **)
 
 let zsign_ext n0 x0 =
-  Z.iter (Z.pred n0) (fun rec0 x1 -> zshiftin (Z.odd x1) (rec0 (Z.div2 x1))) (fun x1 ->
+  Z.iter (Z.pred n0) (fun rec0 x1 ->
+    zshiftin (Z.odd x1) (rec0 (Z.div2 x1))) (fun x1 ->
     match match Z.odd x1 with
           | True -> proj_sumbool (zlt Z0 n0)
           | False -> False with
@@ -969,9 +1018,10 @@ let rec p_is_power2 = function
 (** val z_is_power2 : z -> z option **)
 
 let z_is_power2 x0 = match x0 with
-| Zpos p -> (match p_is_power2 p with
-             | True -> Some (Z.log2 x0)
-             | False -> None)
+| Zpos p ->
+  (match p_is_power2 p with
+   | True -> Some (Z.log2 x0)
+   | False -> None)
 | _ -> None
 
 (** val zsize : z -> z **)
@@ -989,11 +1039,6 @@ type binary_float =
 type binary32 = binary_float
 
 type binary64 = binary_float
-
-(** val ptr64 : bool **)
-
-let ptr64 =
-  True
 
 type comparison0 =
 | Ceq
@@ -1060,9 +1105,10 @@ module Make =
   | Z0 -> Z0
   | Zpos p -> p_mod_two_p p wordsize
   | Zneg p ->
-    let r0 = p_mod_two_p p wordsize in (match zeq r0 Z0 with
-                                        | Left -> Z0
-                                        | Right -> Z.sub modulus r0)
+    let r0 = p_mod_two_p p wordsize in
+    (match zeq r0 Z0 with
+     | Left -> Z0
+     | Right -> Z.sub modulus r0)
 
   (** val unsigned : int -> z **)
 
@@ -1072,9 +1118,10 @@ module Make =
   (** val signed : int -> z **)
 
   let signed n0 =
-    let x0 = unsigned n0 in (match zlt x0 half_modulus with
-                             | Left -> x0
-                             | Right -> Z.sub x0 modulus)
+    let x0 = unsigned n0 in
+    (match zlt x0 half_modulus with
+     | Left -> x0
+     | Right -> Z.sub x0 modulus)
 
   (** val repr : z -> int **)
 
@@ -1212,13 +1259,17 @@ module Make =
 
   let rol x0 y0 =
     let n0 = Z.modulo (unsigned y0) zwordsize in
-    repr (Z.coq_lor (Z.shiftl (unsigned x0) n0) (Z.shiftr (unsigned x0) (Z.sub zwordsize n0)))
+    repr
+      (Z.coq_lor (Z.shiftl (unsigned x0) n0)
+        (Z.shiftr (unsigned x0) (Z.sub zwordsize n0)))
 
   (** val ror : int -> int -> int **)
 
   let ror x0 y0 =
     let n0 = Z.modulo (unsigned y0) zwordsize in
-    repr (Z.coq_lor (Z.shiftr (unsigned x0) n0) (Z.shiftl (unsigned x0) (Z.sub zwordsize n0)))
+    repr
+      (Z.coq_lor (Z.shiftr (unsigned x0) n0)
+        (Z.shiftl (unsigned x0) (Z.sub zwordsize n0)))
 
   (** val rolm : int -> int -> int -> int **)
 
@@ -1250,7 +1301,9 @@ module Make =
   (** val add_carry : int -> int -> int -> int **)
 
   let add_carry x0 y0 cin =
-    match zlt (Z.add (Z.add (unsigned x0) (unsigned y0)) (unsigned cin)) modulus with
+    match zlt
+            (Z.add (Z.add (unsigned x0) (unsigned y0)) (unsigned cin))
+            modulus with
     | Left -> zero
     | Right -> one
 
@@ -1267,7 +1320,9 @@ module Make =
   (** val sub_borrow : int -> int -> int -> int **)
 
   let sub_borrow x0 y0 bin =
-    match zlt (Z.sub (Z.sub (unsigned x0) (unsigned y0)) (unsigned bin)) Z0 with
+    match zlt
+            (Z.sub (Z.sub (unsigned x0) (unsigned y0)) (unsigned bin))
+            Z0 with
     | Left -> one
     | Right -> zero
 
@@ -1347,7 +1402,10 @@ module Make =
     match eq_dec d zero with
     | Left -> None
     | Right ->
-      let Pair (q, r0) = Z.div_eucl (Z.add (Z.mul (unsigned nhi) modulus) (unsigned nlo)) (unsigned d)
+      let Pair (q, r0) =
+        Z.div_eucl
+          (Z.add (Z.mul (unsigned nhi) modulus) (unsigned nlo))
+          (unsigned d)
       in
       (match zle q max_unsigned with
        | Left -> Some (Pair ((repr q), (repr r0)))
@@ -1359,7 +1417,10 @@ module Make =
     match eq_dec d zero with
     | Left -> None
     | Right ->
-      let Pair (q, r0) = Z.quotrem (Z.add (Z.mul (signed nhi) modulus) (unsigned nlo)) (signed d) in
+      let Pair (q, r0) =
+        Z.quotrem (Z.add (Z.mul (signed nhi) modulus) (unsigned nlo))
+          (signed d)
+      in
       (match match proj_sumbool (zle min_signed q) with
              | True -> proj_sumbool (zle q max_signed)
              | False -> False with
@@ -1370,12 +1431,14 @@ module Make =
 
   let divs_from_divu x0 y0 =
     match lt x0 zero with
-    | True -> (match lt y0 zero with
-               | True -> divu (neg x0) (neg y0)
-               | False -> neg (divu (neg x0) y0))
-    | False -> (match lt y0 zero with
-                | True -> neg (divu x0 (neg y0))
-                | False -> divu x0 y0)
+    | True ->
+      (match lt y0 zero with
+       | True -> divu (neg x0) (neg y0)
+       | False -> neg (divu (neg x0) y0))
+    | False ->
+      (match lt y0 zero with
+       | True -> neg (divu x0 (neg y0))
+       | False -> divu x0 y0)
 
   (** val testbit : int -> z -> bool **)
 
@@ -1420,7 +1483,8 @@ module Make =
   (** val bitfield_insert : z -> z -> int -> int -> int **)
 
   let bitfield_insert pos width n0 p =
-    let mask0 = shl (repr (Z.sub (two_p width) (Zpos XH))) (repr pos) in
+    let mask0 = shl (repr (Z.sub (two_p width) (Zpos XH))) (repr pos)
+    in
     coq_or (shl (zero_ext width p) (repr pos)) (coq_and n0 (not mask0))
  end
 
@@ -1429,8 +1493,8 @@ module Wordsize_32 =
   (** val wordsize : nat **)
 
   let wordsize =
-    S (S (S (S (S (S (S (S (S (S (S (S (S (S (S (S (S (S (S (S (S (S (S (S (S (S (S (S (S (S (S (S
-      O)))))))))))))))))))))))))))))))
+    S (S (S (S (S (S (S (S (S (S (S (S (S (S (S (S (S (S (S (S (S (S
+      (S (S (S (S (S (S (S (S (S (S O)))))))))))))))))))))))))))))))
  end
 
 module Int = Make(Wordsize_32)
@@ -1451,55 +1515,10 @@ module Int64 =
     (* singleton inductive, whose constructor was mkint *)
  end
 
-module Wordsize_Ptrofs =
- struct
-  (** val wordsize : nat **)
-
-  let wordsize =
-    match ptr64 with
-    | True ->
-      S (S (S (S (S (S (S (S (S (S (S (S (S (S (S (S (S (S (S (S (S (S (S (S (S (S (S (S (S (S (S (S
-        (S (S (S (S (S (S (S (S (S (S (S (S (S (S (S (S (S (S (S (S (S (S (S (S (S (S (S (S (S (S (S
-        (S O)))))))))))))))))))))))))))))))))))))))))))))))))))))))))))))))
-    | False ->
-      S (S (S (S (S (S (S (S (S (S (S (S (S (S (S (S (S (S (S (S (S (S (S (S (S (S (S (S (S (S (S (S
-        O)))))))))))))))))))))))))))))))
- end
-
 module Ptrofs =
  struct
-  (** val wordsize : nat **)
-
-  let wordsize =
-    Wordsize_Ptrofs.wordsize
-
-  (** val modulus : z **)
-
-  let modulus =
-    two_power_nat wordsize
-
   type int = z
     (* singleton inductive, whose constructor was mkint *)
-
-  (** val coq_Z_mod_modulus : z -> z **)
-
-  let coq_Z_mod_modulus = function
-  | Z0 -> Z0
-  | Zpos p -> p_mod_two_p p wordsize
-  | Zneg p ->
-    let r0 = p_mod_two_p p wordsize in (match zeq r0 Z0 with
-                                        | Left -> Z0
-                                        | Right -> Z.sub modulus r0)
-
-  (** val repr : z -> int **)
-
-  let repr =
-    coq_Z_mod_modulus
-
-  (** val of_ints : Int.int -> int **)
-
-  let of_ints x0 =
-    repr (Int.signed x0)
  end
 
 module PTree =
@@ -1636,7 +1655,8 @@ module PMap =
     | Some x0 -> x0
     | None -> fst m
 
-  (** val set : positive -> 'a1 -> 'a1 t -> ('a1, 'a1 PTree.tree) prod **)
+  (** val set :
+      positive -> 'a1 -> 'a1 t -> ('a1, 'a1 PTree.tree) prod **)
 
   let set i x0 m =
     Pair ((fst m), (PTree.set i x0 (snd m)))
@@ -1749,9 +1769,16 @@ type rettype =
 | Tint16unsigned
 | Tvoid
 
-type calling_convention = { cc_vararg : z option; cc_unproto : bool; cc_structret : bool }
+type calling_convention = { cc_vararg : z option; cc_unproto : 
+                            bool; cc_structret : bool }
 
-type signature = { sig_args : typ list; sig_res : rettype; sig_cc : calling_convention }
+(** val cc_default : calling_convention **)
+
+let cc_default =
+  { cc_vararg = None; cc_unproto = False; cc_structret = False }
+
+type signature = { sig_args : typ list; sig_res : rettype;
+                   sig_cc : calling_convention }
 
 type memory_chunk =
 | Mbool
@@ -1776,8 +1803,8 @@ type init_data =
 | Init_space of z
 | Init_addrof of ident * Ptrofs.int
 
-type 'v globvar = { gvar_info : 'v; gvar_init : init_data list; gvar_readonly : bool;
-                    gvar_volatile : bool }
+type 'v globvar = { gvar_info : 'v; gvar_init : init_data list;
+                    gvar_readonly : bool; gvar_volatile : bool }
 
 type ('f, 'v) globdef =
 | Gfun of 'f
@@ -1840,8 +1867,9 @@ type members = member list
 type composite_definition =
 | Composite of ident * struct_or_union * members * attr
 
-type composite = { co_su : struct_or_union; co_members : members; co_attr : attr; co_sizeof : 
-                   z; co_alignof : z; co_rank : nat }
+type composite = { co_su : struct_or_union; co_members : members;
+                   co_attr : attr; co_sizeof : z; co_alignof : 
+                   z; co_rank : nat }
 
 type composite_env = composite PTree.t
 
@@ -1853,9 +1881,11 @@ type 'f fundef =
 | Internal of 'f
 | External of external_function * typelist * type0 * calling_convention
 
-type 'f program = { prog_defs : (ident, ('f fundef, type0) globdef) prod list;
-                    prog_public : ident list; prog_main : ident;
-                    prog_types : composite_definition list; prog_comp_env : composite_env }
+type 'f program = { prog_defs : (ident, ('f fundef, type0) globdef)
+                                prod list; prog_public : ident list;
+                    prog_main : ident;
+                    prog_types : composite_definition list;
+                    prog_comp_env : composite_env }
 
 type block = positive
 
@@ -1889,7 +1919,8 @@ type perm_kind =
 module Mem =
  struct
   type mem' = { mem_contents : memval ZMap.t PMap.t;
-                mem_access : (z -> perm_kind -> permission option) PMap.t; nextblock : block }
+                mem_access : (z -> perm_kind -> permission option)
+                             PMap.t; nextblock : block }
 
   type mem = mem'
  end
@@ -1908,7 +1939,8 @@ type primitive_type =
 | Tint1 of intsize * signedness * attr
 | Tlong1 of signedness * attr
 
-type basic_type = primitive_type
+type basic_type =
+  primitive_type
   (* singleton inductive, whose constructor was Bprim *)
 
 type type1 =
@@ -1916,13 +1948,15 @@ type type1 =
 | Reftype of ident * basic_type * attr
 | Ftype of type1 list * effect * type1
 
-(** val transBeePL_types : (type1 -> type0 res) -> type1 list -> typelist res **)
+(** val transBeePL_types :
+    (type1 -> type0 res) -> type1 list -> typelist res **)
 
 let rec transBeePL_types transBeePL_type0 = function
 | Nil -> OK Tnil
 | Cons (t0, ts0) ->
   bind (transBeePL_type0 t0) (fun ct ->
-    bind (transBeePL_types transBeePL_type0 ts0) (fun cts -> OK (Tcons (ct, cts))))
+    bind (transBeePL_types transBeePL_type0 ts0) (fun cts -> OK (Tcons
+      (ct, cts))))
 
 (** val typelist_list_type : typelist -> type0 list **)
 
@@ -1935,7 +1969,9 @@ let rec typelist_list_type = function
 let rec transBeePL_type = function
 | Ptype t1 ->
   (match t1 with
-   | Tunit -> OK (Tint0 (I8, Unsigned, { attr_volatile = False; attr_alignas = (Some (Npos XH)) }))
+   | Tunit ->
+     OK (Tint0 (I8, Unsigned, { attr_volatile = False; attr_alignas =
+       (Some (Npos XH)) }))
    | Tint1 (sz, s, a) -> OK (Tint0 (sz, s, a))
    | Tlong1 (s, a) -> OK (Tlong0 (s, a)))
 | Reftype (_, bt, a) ->
@@ -1945,8 +1981,9 @@ let rec transBeePL_type = function
    | Tlong1 (s, a0) -> OK (Tpointer ((Tlong0 (s, a0)), a0)))
 | Ftype (ts, _, t1) ->
   bind (transBeePL_types transBeePL_type ts) (fun ats ->
-    bind (transBeePL_type t1) (fun rt -> OK (Tfunction (ats, rt, { cc_vararg = (Some
-      (Z.of_nat (length ts))); cc_unproto = False; cc_structret = False }))))
+    bind (transBeePL_type t1) (fun rt -> OK (Tfunction (ats, rt,
+      { cc_vararg = (Some (Z.of_nat (length ts))); cc_unproto = False;
+      cc_structret = False }))))
 
 (** val unzip1 : ('a1, 'a2) prod list -> 'a1 list **)
 
@@ -2003,11 +2040,6 @@ type constant =
 | ConsLong of Int64.int
 | ConsUnit
 
-type gconstant =
-| Gvalue of constant
-| Gloc of positive
-| Gspace of z
-
 type vinfo = { vname : ident; vtype : type1 }
 
 type linfo = { lname : ident; ltype : type1; lbitfield : bitfield }
@@ -2018,11 +2050,13 @@ type value =
 | Vint64 of Int64.int
 | Vloc of positive * Ptrofs.int
 
-(** val extract_list_rvtypes : vinfo list -> (ident, type1) prod list **)
+(** val extract_list_rvtypes :
+    vinfo list -> (ident, type1) prod list **)
 
 let rec extract_list_rvtypes = function
 | Nil -> Nil
-| Cons (x0, xs) -> Cons ((Pair (x0.vname, x0.vtype)), (extract_list_rvtypes xs))
+| Cons (x0, xs) ->
+  Cons ((Pair (x0.vname, x0.vtype)), (extract_list_rvtypes xs))
 
 type builtin =
 | Ref
@@ -2033,6 +2067,7 @@ type builtin =
 | Run of Mem.mem
 
 type expr =
+| Val of value * type1
 | Var of vinfo
 | Const of constant * type1
 | App of ident option * expr * expr list * type1
@@ -2046,6 +2081,7 @@ type expr =
 (** val typeof_expr : expr -> type1 **)
 
 let typeof_expr = function
+| Val (_, t0) -> t0
 | Var x0 -> x0.vtype
 | Const (_, t0) -> t0
 | App (_, _, _, t0) -> t0
@@ -2056,21 +2092,32 @@ let typeof_expr = function
 | Addr (l, _) -> l.ltype
 | Hexpr (_, _, t0) -> t0
 
-type fun_decl = { fname : ident; args : vinfo list; lvars : vinfo list; rtype : type1; body : expr }
+type function0 = { fn_return : type1;
+                   fn_callconv : calling_convention;
+                   fn_args : vinfo list; fn_vars : vinfo list;
+                   fn_body : expr }
 
-type glob_decl = { gname : ident; gtype : type1; gval : gconstant list }
+type fundef0 =
+| Internal0 of function0
+| External0
 
-type func = fun_decl
-  (* singleton inductive, whose constructor was Fun *)
+type init_data0 =
+| Init_int0 of Int.int
+| Init_int1 of Int.int
+| Init_int2 of Int.int
+| Init_int3 of Int64.int
 
-type globv = glob_decl
-  (* singleton inductive, whose constructor was Glob *)
+type globvar0 = { gvar_info0 : type1; gvar_init0 : init_data0 list;
+                  gvar_readonly0 : bool; gvar_volatile0 : bool }
 
-type decl =
-| Fdecl of func
-| Gvdecl of globv
+type globdef0 =
+| Gfun0 of fundef0
+| Gvar0 of globvar0
 
-type program0 = { bprog_defs : (positive, decl) prod list; bprog_main : positive }
+type program0 = { prog_defs0 : (ident, globdef0) prod list;
+                  prog_public0 : ident list; prog_main0 : ident;
+                  prog_types0 : composite_definition list;
+                  prog_comp_env0 : composite_env }
 
 (** val transBeePL_value_cvalue : value -> val0 **)
 
@@ -2127,19 +2174,25 @@ and labeled_statements =
 | LSnil
 | LScons of z option * statement * labeled_statements
 
-type function0 = { fn_return : type0; fn_callconv : calling_convention;
-                   fn_params : (ident, type0) prod list; fn_vars : (ident, type0) prod list;
-                   fn_body : statement }
+type function1 = { fn_return0 : type0;
+                   fn_callconv0 : calling_convention;
+                   fn_params : (ident, type0) prod list;
+                   fn_vars0 : (ident, type0) prod list;
+                   fn_body0 : statement }
 
-type program1 = function0 program
+type fundef1 = function1 fundef
 
-(** val transBeePL_expr_exprs : (expr -> expr0 res) -> expr list -> exprlist res **)
+type program1 = function1 program
+
+(** val transBeePL_expr_exprs :
+    (expr -> expr0 res) -> expr list -> exprlist res **)
 
 let rec transBeePL_expr_exprs transBeePL_expr_expr0 = function
 | Nil -> OK Enil
 | Cons (e, es0) ->
   bind (transBeePL_expr_expr0 e) (fun ce ->
-    bind (transBeePL_expr_exprs transBeePL_expr_expr0 es0) (fun ces -> OK (Econs (ce, ces))))
+    bind (transBeePL_expr_exprs transBeePL_expr_expr0 es0) (fun ces ->
+      OK (Econs (ce, ces))))
 
 (** val exprlist_list_expr : exprlist -> expr0 list **)
 
@@ -2155,12 +2208,20 @@ let default_expr =
 (** val transBeePL_expr_expr : expr -> expr0 res **)
 
 let rec transBeePL_expr_expr = function
-| Var x0 -> bind (transBeePL_type x0.vtype) (fun xt -> OK (Evar (x0.vname, xt)))
+| Val (v, t0) ->
+  bind (transBeePL_type t0) (fun vt -> OK (Eval
+    ((transBeePL_value_cvalue v), vt)))
+| Var x0 ->
+  bind (transBeePL_type x0.vtype) (fun xt -> OK (Evar (x0.vname, xt)))
 | Const (c, t0) ->
   (match c with
-   | ConsInt i -> bind (transBeePL_type t0) (fun it -> OK (Eval ((Vint i), it)))
-   | ConsLong i -> bind (transBeePL_type t0) (fun it -> OK (Eval ((Vlong i), it)))
-   | ConsUnit -> bind (transBeePL_type t0) (fun ut -> OK (Eval ((Vint (Int.repr Z0)), ut))))
+   | ConsInt i ->
+     bind (transBeePL_type t0) (fun it -> OK (Eval ((Vint i), it)))
+   | ConsLong i ->
+     bind (transBeePL_type t0) (fun it -> OK (Eval ((Vlong i), it)))
+   | ConsUnit ->
+     bind (transBeePL_type t0) (fun ut -> OK (Eval ((Vint
+       (Int.repr Z0)), ut))))
 | App (_, e0, es, t0) ->
   bind (transBeePL_expr_expr e0) (fun ce ->
     bind (transBeePL_expr_exprs transBeePL_expr_expr es) (fun ces ->
@@ -2169,40 +2230,45 @@ let rec transBeePL_expr_expr = function
   (match b with
    | Ref ->
      bind (transBeePL_expr_exprs transBeePL_expr_expr es) (fun ces ->
-       bind (transBeePL_type t0) (fun ct -> OK (Eaddrof ((hd default_expr (exprlist_list_expr ces)),
-         ct))))
+       bind (transBeePL_type t0) (fun ct -> OK (Eaddrof
+         ((hd default_expr (exprlist_list_expr ces)), ct))))
    | Deref ->
      bind (transBeePL_expr_exprs transBeePL_expr_expr es) (fun ces ->
-       bind (transBeePL_type t0) (fun ct -> OK (Ederef ((hd default_expr (exprlist_list_expr ces)),
-         ct))))
+       bind (transBeePL_type t0) (fun ct -> OK (Ederef
+         ((hd default_expr (exprlist_list_expr ces)), ct))))
    | Massgn ->
      bind (transBeePL_expr_exprs transBeePL_expr_expr es) (fun ces ->
-       bind (transBeePL_type t0) (fun ct -> OK (Eassign ((hd default_expr (exprlist_list_expr ces)),
+       bind (transBeePL_type t0) (fun ct -> OK (Eassign
+         ((hd default_expr (exprlist_list_expr ces)),
          (hd default_expr (tl (exprlist_list_expr ces))), ct))))
    | Uop o ->
      bind (transBeePL_expr_exprs transBeePL_expr_expr es) (fun ces ->
-       bind (transBeePL_type t0) (fun ct -> OK (Eunop (o, (hd default_expr (exprlist_list_expr ces)),
-         ct))))
+       bind (transBeePL_type t0) (fun ct -> OK (Eunop (o,
+         (hd default_expr (exprlist_list_expr ces)), ct))))
    | Bop o ->
      bind (transBeePL_expr_exprs transBeePL_expr_expr es) (fun ces ->
        bind (transBeePL_type t0) (fun ct -> OK (Ebinop (o,
-         (hd default_expr (exprlist_list_expr ces)), (hd default_expr (tl (exprlist_list_expr ces))),
-         ct))))
+         (hd default_expr (exprlist_list_expr ces)),
+         (hd default_expr (tl (exprlist_list_expr ces))), ct))))
    | Run _ -> OK (Eval (Vundef, Tvoid0)))
 | Bind (x0, t0, e0, e', t') ->
   bind (transBeePL_type t0) (fun ct ->
     bind (transBeePL_expr_expr e0) (fun ce ->
       bind (transBeePL_expr_expr e') (fun ce' ->
-        bind (transBeePL_type t') (fun ct' -> OK (Ecomma ((Eassign ((Evar (x0, ct)), ce, ct)), ce',
-          ct'))))))
+        bind (transBeePL_type t') (fun ct' -> OK (Ecomma ((Eassign
+          ((Evar (x0, ct)), ce, ct)), ce', ct'))))))
 | Cond (e0, e', e'', t0) ->
   bind (transBeePL_expr_expr e0) (fun ce ->
     bind (transBeePL_expr_expr e') (fun ce' ->
       bind (transBeePL_expr_expr e'') (fun ce'' ->
-        bind (transBeePL_type t0) (fun ct -> OK (Econdition (ce, ce', ce'', ct))))))
-| Unit t0 -> bind (transBeePL_type t0) (fun ct -> OK (Eval ((transBeePL_value_cvalue Vunit), ct)))
+        bind (transBeePL_type t0) (fun ct -> OK (Econdition (ce, ce',
+          ce'', ct))))))
+| Unit t0 ->
+  bind (transBeePL_type t0) (fun ct -> OK (Eval
+    ((transBeePL_value_cvalue Vunit), ct)))
 | Addr (l, ofs) ->
-  bind (transBeePL_type l.ltype) (fun ct -> OK (Eloc (l.lname, ofs, l.lbitfield, ct)))
+  bind (transBeePL_type l.ltype) (fun ct -> OK (Eloc (l.lname, ofs,
+    l.lbitfield, ct)))
 | Hexpr (_, _, _) -> OK (Eval (Vundef, Tvoid0))
 
 (** val check_var_const : expr -> bool **)
@@ -2215,8 +2281,12 @@ let check_var_const = function
 (** val transBeePL_expr_st : expr -> statement res **)
 
 let transBeePL_expr_st = function
+| Val (v, t0) ->
+  bind (transBeePL_type t0) (fun vt -> OK (Sreturn (Some (Eval
+    ((transBeePL_value_cvalue v), vt)))))
 | Var x0 ->
-  bind (transBeePL_type x0.vtype) (fun ct -> OK (Sreturn (Some (Evalof ((Evar (x0.vname, ct)), ct)))))
+  bind (transBeePL_type x0.vtype) (fun ct -> OK (Sreturn (Some (Evalof
+    ((Evar (x0.vname, ct)), ct)))))
 | Const (c, t0) ->
   bind (transBeePL_type t0) (fun ct -> OK (Sreturn (Some (Evalof
     ((match c with
@@ -2226,7 +2296,8 @@ let transBeePL_expr_st = function
 | App (_, e0, es, t0) ->
   bind (transBeePL_expr_expr e0) (fun ce ->
     bind (transBeePL_expr_exprs transBeePL_expr_expr es) (fun ces ->
-      bind (transBeePL_type t0) (fun ct -> OK (Sdo (Ecall (ce, ces, ct))))))
+      bind (transBeePL_type t0) (fun ct -> OK (Sdo (Ecall (ce, ces,
+        ct))))))
 | Prim (b, es, t0) ->
   (match b with
    | Ref ->
@@ -2249,8 +2320,8 @@ let transBeePL_expr_st = function
    | Bop o ->
      bind (transBeePL_expr_exprs transBeePL_expr_expr es) (fun ces ->
        bind (transBeePL_type t0) (fun ct -> OK (Sdo (Ebinop (o,
-         (hd default_expr (exprlist_list_expr ces)), (hd default_expr (tl (exprlist_list_expr ces))),
-         ct)))))
+         (hd default_expr (exprlist_list_expr ces)),
+         (hd default_expr (tl (exprlist_list_expr ces))), ct)))))
    | Run _ -> OK (Sdo (Eval (Vundef, Tvoid0))))
 | Bind (x0, t0, e0, e', t') ->
   (match e' with
@@ -2259,18 +2330,20 @@ let transBeePL_expr_st = function
        bind (transBeePL_expr_expr e') (fun ce' ->
          bind (transBeePL_type t0) (fun ct ->
            bind (transBeePL_type t') (fun _ ->
-             bind (transBeePL_type (typeof_expr e')) (fun rt -> OK (Ssequence ((Sdo (Eassign ((Evar
-               (x0, ct)), ce, Tvoid0))), (Sreturn (Some (Evalof (ce', rt)))))))))))
+             bind (transBeePL_type (typeof_expr e')) (fun rt -> OK
+               (Ssequence ((Sdo (Eassign ((Evar (x0, ct)), ce,
+               Tvoid0))), (Sreturn (Some (Evalof (ce', rt)))))))))))
    | Const (_, t1) ->
      bind (transBeePL_type t1) (fun ct ->
        bind (transBeePL_expr_expr e0) (fun ce ->
-         bind (transBeePL_expr_expr e') (fun ce' -> OK (Ssequence ((Sdo (Eassign ((Evar (x0, ct)),
-           ce, Tvoid0))), (Sreturn (Some ce')))))))
+         bind (transBeePL_expr_expr e') (fun ce' -> OK (Ssequence
+           ((Sdo (Eassign ((Evar (x0, ct)), ce, Tvoid0))), (Sreturn
+           (Some ce')))))))
    | _ ->
      bind (transBeePL_type t0) (fun ct ->
        bind (transBeePL_expr_expr e0) (fun ce ->
-         bind (transBeePL_expr_expr e') (fun ce' -> OK (Ssequence ((Sdo (Eassign ((Evar (x0, ct)),
-           ce, Tvoid0))), (Sdo ce')))))))
+         bind (transBeePL_expr_expr e') (fun ce' -> OK (Ssequence
+           ((Sdo (Eassign ((Evar (x0, ct)), ce, Tvoid0))), (Sdo ce')))))))
 | Cond (e0, e', e'', t') ->
   bind (transBeePL_expr_expr e0) (fun ce ->
     bind (transBeePL_expr_expr e') (fun ce' ->
@@ -2280,80 +2353,137 @@ let transBeePL_expr_st = function
                 | True -> check_var_const e''
                 | False -> False with
           | True ->
-            OK (Sifthenelse (ce, (Sreturn (Some (Evalof (ce', ct')))), (Sreturn (Some (Evalof (ce'',
-              ct'))))))
+            OK (Sifthenelse (ce, (Sreturn (Some (Evalof (ce', ct')))),
+              (Sreturn (Some (Evalof (ce'', ct'))))))
           | False ->
             (match check_var_const e' with
-             | True -> OK (Sifthenelse (ce, (Sreturn (Some (Evalof (ce', ct')))), (Sdo ce'')))
+             | True ->
+               OK (Sifthenelse (ce, (Sreturn (Some (Evalof (ce',
+                 ct')))), (Sdo ce'')))
              | False ->
                (match check_var_const e'' with
-                | True -> OK (Sifthenelse (ce, (Sdo ce'), (Sreturn (Some (Evalof (ce'', ct'))))))
+                | True ->
+                  OK (Sifthenelse (ce, (Sdo ce'), (Sreturn (Some
+                    (Evalof (ce'', ct'))))))
                 | False -> OK (Sifthenelse (ce, (Sdo ce'), (Sdo ce'')))))))))
 | Unit t0 ->
-  bind (transBeePL_type t0) (fun ct -> OK (Sreturn (Some (Evalof ((Eval
-    ((transBeePL_value_cvalue Vunit), ct)), ct)))))
+  bind (transBeePL_type t0) (fun ct -> OK (Sreturn (Some (Evalof
+    ((Eval ((transBeePL_value_cvalue Vunit), ct)), ct)))))
 | Addr (l, ofs) ->
-  bind (transBeePL_type l.ltype) (fun ct -> OK (Sdo (Eloc (l.lname, ofs, l.lbitfield, ct))))
+  bind (transBeePL_type l.ltype) (fun ct -> OK (Sdo (Eloc (l.lname,
+    ofs, l.lbitfield, ct))))
 | Hexpr (_, _, _) -> OK (Sdo (Eval (Vundef, Tvoid0)))
 
-(** val default_cc : fun_decl -> calling_convention **)
+(** val transBeePL_function_function : function0 -> function1 res **)
 
-let default_cc fd =
-  { cc_vararg = (Some (Z.of_nat (length fd.args))); cc_unproto = False; cc_structret = False }
+let transBeePL_function_function fd =
+  bind (transBeePL_type fd.fn_return) (fun crt ->
+    bind
+      (transBeePL_types transBeePL_type
+        (unzip2 (extract_list_rvtypes fd.fn_args))) (fun pt ->
+      bind
+        (transBeePL_types transBeePL_type
+          (unzip2 (extract_list_rvtypes fd.fn_vars))) (fun vt ->
+        bind (transBeePL_expr_st fd.fn_body) (fun fbody -> OK
+          { fn_return0 = crt; fn_callconv0 = cc_default; fn_params =
+          (zip (unzip1 (extract_list_rvtypes fd.fn_args))
+            (typelist_list_type pt)); fn_vars0 =
+          (zip (unzip1 (extract_list_rvtypes fd.fn_vars))
+            (typelist_list_type vt)); fn_body0 = fbody }))))
 
-(** val beePLfd_function : fun_decl -> function0 fundef res **)
+(** val transBeePL_fundef_fundef : fundef0 -> fundef1 res **)
 
-let beePLfd_function fd =
-  bind (transBeePL_type fd.rtype) (fun crt ->
-    bind (transBeePL_types transBeePL_type (unzip2 (extract_list_rvtypes fd.args))) (fun pt ->
-      bind (transBeePL_types transBeePL_type (unzip2 (extract_list_rvtypes fd.lvars))) (fun vt ->
-        bind (transBeePL_expr_st fd.body) (fun fbody -> OK (Internal { fn_return = crt; fn_callconv =
-          (default_cc fd); fn_params =
-          (zip (unzip1 (extract_list_rvtypes fd.args)) (typelist_list_type pt)); fn_vars =
-          (zip (unzip1 (extract_list_rvtypes fd.lvars)) (typelist_list_type vt)); fn_body = fbody })))))
+let transBeePL_fundef_fundef = function
+| Internal0 f ->
+  bind (transBeePL_function_function f) (fun tf -> OK (Internal tf))
+| External0 ->
+  Error (Cons ((MSG (String ((Ascii (True, False, True, False, False,
+    False, True, False)), (String ((Ascii (False, False, False, True,
+    True, True, True, False)), (String ((Ascii (False, False, True,
+    False, True, True, True, False)), (String ((Ascii (True, False,
+    True, False, False, True, True, False)), (String ((Ascii (False,
+    True, False, False, True, True, True, False)), (String ((Ascii
+    (False, True, True, True, False, True, True, False)), (String
+    ((Ascii (True, False, False, False, False, True, True, False)),
+    (String ((Ascii (False, False, True, True, False, True, True,
+    False)), (String ((Ascii (False, False, False, False, False, True,
+    False, False)), (String ((Ascii (False, True, True, False, False,
+    True, True, False)), (String ((Ascii (True, False, True, False,
+    True, True, True, False)), (String ((Ascii (False, True, True,
+    True, False, True, True, False)), (String ((Ascii (True, True,
+    False, False, False, True, True, False)), (String ((Ascii (False,
+    False, True, False, True, True, True, False)), (String ((Ascii
+    (True, False, False, True, False, True, True, False)), (String
+    ((Ascii (True, True, True, True, False, True, True, False)),
+    (String ((Ascii (False, True, True, True, False, True, True,
+    False)), (String ((Ascii (False, False, False, False, False, True,
+    False, False)), (String ((Ascii (False, True, True, True, False,
+    True, True, False)), (String ((Ascii (True, True, True, True,
+    False, True, True, False)), (String ((Ascii (False, False, True,
+    False, True, True, True, False)), (String ((Ascii (False, False,
+    False, False, False, True, False, False)), (String ((Ascii (True,
+    True, False, False, True, True, True, False)), (String ((Ascii
+    (True, False, True, False, True, True, True, False)), (String
+    ((Ascii (False, False, False, False, True, True, True, False)),
+    (String ((Ascii (False, False, False, False, True, True, True,
+    False)), (String ((Ascii (True, True, True, True, False, True,
+    True, False)), (String ((Ascii (False, True, False, False, True,
+    True, True, False)), (String ((Ascii (False, False, True, False,
+    True, True, True, False)), (String ((Ascii (True, False, True,
+    False, False, True, True, False)), (String ((Ascii (False, False,
+    True, False, False, True, True, False)),
+    EmptyString))))))))))))))))))))))))))))))))))))))))))))))))))))))))))))))),
+    Nil))
 
-(** val gconstant_init_data : gconstant -> init_data **)
+(** val transBeePL_init_data_init_data : init_data0 -> init_data **)
 
-let gconstant_init_data = function
-| Gvalue c ->
-  (match c with
-   | ConsInt i -> Init_int32 i
-   | ConsLong i -> Init_int64 i
-   | ConsUnit -> Init_int32 (Int.repr Z0))
-| Gloc p -> Init_addrof (p, (Ptrofs.of_ints (Int.repr Z0)))
-| Gspace z0 -> Init_space z0
+let transBeePL_init_data_init_data = function
+| Init_int0 i -> Init_int8 i
+| Init_int1 i -> Init_int16 i
+| Init_int2 i -> Init_int32 i
+| Init_int3 i -> Init_int64 i
 
-(** val gconstants_init_datas : gconstant list -> init_data list **)
+(** val transBeePL_init_datas_init_datas :
+    init_data0 list -> init_data list **)
 
-let rec gconstants_init_datas = function
+let rec transBeePL_init_datas_init_datas = function
 | Nil -> Nil
-| Cons (g, gs0) -> Cons ((gconstant_init_data g), (gconstants_init_datas gs0))
+| Cons (g, gs0) ->
+  Cons ((transBeePL_init_data_init_data g),
+    (transBeePL_init_datas_init_datas gs0))
 
-(** val beePLgd_gd : glob_decl -> type0 globvar res **)
+(** val transBeePLglobvar_globvar : globvar0 -> type0 globvar res **)
 
-let beePLgd_gd gv =
-  bind (transBeePL_type gv.gtype) (fun gvt -> OK { gvar_info = gvt; gvar_init =
-    (gconstants_init_datas gv.gval); gvar_readonly = False; gvar_volatile = False })
+let transBeePLglobvar_globvar gv =
+  bind (transBeePL_type gv.gvar_info0) (fun gvt -> OK { gvar_info =
+    gvt; gvar_init = (transBeePL_init_datas_init_datas gv.gvar_init0);
+    gvar_readonly = False; gvar_volatile = False })
 
-(** val beePLdecl_gdef : decl -> (function0 fundef, type0) globdef res **)
+(** val transBeePL_globdef_globdef :
+    globdef0 -> (fundef1, type0) globdef res **)
 
-let beePLdecl_gdef = function
-| Fdecl f -> bind (beePLfd_function f) (fun cfd -> OK (Gfun cfd))
-| Gvdecl g -> bind (beePLgd_gd g) (fun gv -> OK (Gvar gv))
+let transBeePL_globdef_globdef = function
+| Gfun0 f -> bind (transBeePL_fundef_fundef f) (fun cf -> OK (Gfun cf))
+| Gvar0 g ->
+  bind (transBeePLglobvar_globvar g) (fun cg -> OK (Gvar cg))
 
-(** val beePLdecls_gdefs : decl list -> (function0 fundef, type0) globdef list res **)
+(** val transBeePL_globdefs_globdefs :
+    globdef0 list -> (fundef1, type0) globdef list res **)
 
-let rec beePLdecls_gdefs = function
+let rec transBeePL_globdefs_globdefs = function
 | Nil -> OK Nil
-| Cons (d, ds0) ->
-  bind (beePLdecl_gdef d) (fun gd -> bind (beePLdecls_gdefs ds0) (fun gds -> OK (Cons (gd, gds))))
+| Cons (d, ds) ->
+  bind (transBeePL_globdef_globdef d) (fun gd ->
+    bind (transBeePL_globdefs_globdefs ds) (fun gds0 -> OK (Cons (gd,
+      gds0))))
 
 (** val beePL_compcert : program0 -> program1 res **)
 
-let beePL_compcert m =
-  bind (beePLdecls_gdefs (unzip2 m.bprog_defs)) (fun cfd -> OK { prog_defs =
-    (zip (unzip1 m.bprog_defs) cfd); prog_public = Nil; prog_main = m.bprog_main; prog_types = Nil;
-    prog_comp_env = PTree.empty })
+let beePL_compcert p =
+  bind (transBeePL_globdefs_globdefs (unzip2 p.prog_defs0))
+    (fun pds -> OK { prog_defs = (zip (unzip1 p.prog_defs0) pds);
+    prog_public = p.prog_public0; prog_main = p.prog_main0;
+    prog_types = p.prog_types0; prog_comp_env = p.prog_comp_env0 })
 
 (** val apply_partial : 'a1 res -> ('a1 -> 'a2 res) -> 'a2 res **)
 
@@ -2371,21 +2501,28 @@ let time _ f =
 
 let transf_beepl_program_csyntax p =
   apply_partial (OK p)
-    (time (String ((Ascii (True, True, False, False, False, False, True, False)), (String ((Ascii
-      (True, True, False, False, True, True, True, False)), (String ((Ascii (True, False, False,
-      True, True, True, True, False)), (String ((Ascii (False, True, True, True, False, True, True,
-      False)), (String ((Ascii (False, False, True, False, True, True, True, False)), (String ((Ascii
-      (True, False, False, False, False, True, True, False)), (String ((Ascii (False, False, False,
-      True, True, True, True, False)), (String ((Ascii (False, False, False, False, False, True,
-      False, False)), (String ((Ascii (True, True, True, False, False, True, True, False)), (String
-      ((Ascii (True, False, True, False, False, True, True, False)), (String ((Ascii (False, True,
-      True, True, False, True, True, False)), (String ((Ascii (True, False, True, False, False, True,
-      True, False)), (String ((Ascii (False, True, False, False, True, True, True, False)), (String
-      ((Ascii (True, False, False, False, False, True, True, False)), (String ((Ascii (False, False,
-      True, False, True, True, True, False)), (String ((Ascii (True, False, False, True, False, True,
-      True, False)), (String ((Ascii (True, True, True, True, False, True, True, False)), (String
-      ((Ascii (False, True, True, True, False, True, True, False)),
-      EmptyString)))))))))))))))))))))))))))))))))))) beePL_compcert)
+    (time (String ((Ascii (True, True, False, False, False, False,
+      True, False)), (String ((Ascii (True, True, False, False, True,
+      True, True, False)), (String ((Ascii (True, False, False, True,
+      True, True, True, False)), (String ((Ascii (False, True, True,
+      True, False, True, True, False)), (String ((Ascii (False, False,
+      True, False, True, True, True, False)), (String ((Ascii (True,
+      False, False, False, False, True, True, False)), (String ((Ascii
+      (False, False, False, True, True, True, True, False)), (String
+      ((Ascii (False, False, False, False, False, True, False,
+      False)), (String ((Ascii (True, True, True, False, False, True,
+      True, False)), (String ((Ascii (True, False, True, False, False,
+      True, True, False)), (String ((Ascii (False, True, True, True,
+      False, True, True, False)), (String ((Ascii (True, False, True,
+      False, False, True, True, False)), (String ((Ascii (False, True,
+      False, False, True, True, True, False)), (String ((Ascii (True,
+      False, False, False, False, True, True, False)), (String ((Ascii
+      (False, False, True, False, True, True, True, False)), (String
+      ((Ascii (True, False, False, True, False, True, True, False)),
+      (String ((Ascii (True, True, True, True, False, True, True,
+      False)), (String ((Ascii (False, True, True, True, False, True,
+      True, False)), EmptyString))))))))))))))))))))))))))))))))))))
+      beePL_compcert)
 
 (** val dattr : attr **)
 
@@ -2415,23 +2552,44 @@ let main =
 (** val main_body : expr **)
 
 let main_body =
-  Bind (x.vname, (Ptype (Tint1 (I32, Unsigned, dattr))), (Const ((ConsInt (Int.repr (Zpos XH))),
-    (Ptype (Tint1 (I32, Unsigned, dattr))))), (Bind (y.vname, (Ptype (Tint1 (I32, Unsigned, dattr))),
-    (Const ((ConsInt (Int.repr (Zpos (XO XH)))), (Ptype (Tint1 (I32, Unsigned, dattr))))), (Bind
-    (r.vname, (Ptype (Tint1 (I32, Unsigned, dattr))), (Prim ((Bop Oadd), (Cons ((Var x), (Cons ((Var
-    y), Nil)))), (Ptype (Tint1 (I32, Unsigned, dattr))))), (Var r), (Ptype (Tint1 (I32, Unsigned,
-    dattr))))), (Ptype Tunit))), (Ptype Tunit))
+  Bind (x.vname, (Ptype (Tint1 (I32, Unsigned, dattr))), (Const
+    ((ConsInt (Int.repr (Zpos XH))), (Ptype (Tint1 (I32, Unsigned,
+    dattr))))), (Bind (y.vname, (Ptype (Tint1 (I32, Unsigned,
+    dattr))), (Const ((ConsInt (Int.repr (Zpos (XO XH)))), (Ptype
+    (Tint1 (I32, Unsigned, dattr))))), (Bind (r.vname, (Ptype (Tint1
+    (I32, Unsigned, dattr))), (Prim ((Bop Oadd), (Cons ((Var x), (Cons
+    ((Var y), Nil)))), (Ptype (Tint1 (I32, Unsigned, dattr))))), (Var
+    r), (Ptype (Tint1 (I32, Unsigned, dattr))))), (Ptype Tunit))),
+    (Ptype Tunit))
 
-(** val f_main : decl **)
+(** val f_main : function0 **)
 
 let f_main =
-  Fdecl { fname = main; args = Nil; lvars = (Cons (x, (Cons (y, (Cons (r, Nil)))))); rtype = (Ptype
-    (Tint1 (I32, Unsigned, dattr))); body = main_body }
+  { fn_return = (Ptype (Tint1 (I32, Unsigned, dattr))); fn_callconv =
+    cc_default; fn_args = Nil; fn_vars = (Cons (x, (Cons (y, (Cons (r,
+    Nil)))))); fn_body = main_body }
+
+(** val composites : composite_definition list **)
+
+let composites =
+  Nil
+
+(** val global_definitions : (ident, globdef0) prod list **)
+
+let global_definitions =
+  Cons ((Pair (main, (Gfun0 (Internal0 f_main)))), Nil)
+
+(** val public_idents : ident list **)
+
+let public_idents =
+  Cons (main, Nil)
 
 (** val example1 : program0 **)
 
 let example1 =
-  { bprog_defs = (Cons ((Pair (main, f_main)), Nil)); bprog_main = main }
+  { prog_defs0 = global_definitions; prog_public0 = public_idents;
+    prog_main0 = main; prog_types0 = composites; prog_comp_env0 =
+    PTree.empty }
 
 (** val tcp1 : program1 res **)
 
